common/Eventsrel.v
@@ -1,0 +1,13 @@
+Require Import Valuesrel.
+Require Import CKLR.
+Require Export Events.
+
+Global Instance external_call_rel R:
+  Monotonic
+    (@external_call)
+    ([] - ==> - ==> k1 list_rel (Val.inject @@ [mi R]) ++> match_mem R ++> - ==>
+     % k1 set_le (<> Val.inject @@ [mi R] * match_mem R)).
+Admitted.
+
+Hint Extern 1 (Transport _ _ _ _ _) =>
+  rel_curry_set_le_transport @external_call : typeclass_instances.
